theories/genericinv.v
@@ -40,17 +40,17 @@ Section genericinv.
   Qed.
 
   Lemma inv_init :
-    inv (λ v x, ⌜⌜ x = ε ⌝⌝ ∗ emp)%I.
+    inv (λ v x, ⌜⌜ x ≡ ε ⌝⌝ ∗ emp)%I.
   Proof.
     exists ∅.
     split.
     - apply empty_wf.
-    - intros v. rewrite pure_sep_holds emp_holds. split.
-      + admit.
-      + admit.
-  Admitted.
+    - intros v. rewrite pure_sep_holds emp_holds.
+      eauto using in_labels_empty, out_edges_empty.
+  Qed.
 
   Lemma inv_exchange (v1 v2 : V) (f f' : V -> multiset L -> hProp V L) :
+    (∀ v, Proper ((≡) ==> (⊣⊢)) (f v)) ->
     (∀ v x, v ≠ v1 ∧ v ≠ v2 -> f v x ⊢ f' v x) ->
     (∀ y, f v1 y ⊢ ∃ l,
       own_out v2 l ∗
@@ -60,7 +60,7 @@ Section genericinv.
           f' v2 ({[ l' ]} ⋅ x))) ->
     inv f -> inv f'.
   Proof.
-    intros Hrest Hexch Hinv.
+    intros Hproper Hrest Hexch Hinv.
     unfold inv in *.
     destruct Hinv as (g & Hwf & Hvs).
     pose proof (Hvs v1) as Hv1.
@@ -84,9 +84,8 @@ Section genericinv.
       solve_map_disjoint.
     }
 
-    assert (∃ x, in_labels g v2 = {[ b ]} ⋅ x) as [x Hx].
-    { admit. }
-      (* by by eapply out_edges_in_labels. *)
+    assert (∃ x, in_labels g v2 ≡ {[ b ]} ⋅ x) as [x Hx].
+      by by eapply out_edges_in_labels.
 
     pose proof (sep_combine _ _ _ _ H3 Hv2 Hdisj) as Hcomb.
     eapply holds_entails in Hcomb. 2: {
@@ -116,7 +115,8 @@ Section genericinv.
     split.
     - apply exchange_wf; eauto.
     - intros v.
-      erewrite exchange_out_edges; erewrite exchange_in_labels; eauto; last by rewrite Hx.
+      erewrite exchange_out_edges.
+      setoid_rewrite exchange_in_labels; eauto.
       repeat case_decide; simplify_eq; eauto.
       + assert (holds (own_out v2 b') {[ v2 := b' ]}) as Hown
           by by apply own_holds.
@@ -132,5 +132,136 @@ Section genericinv.
         * iIntros "[H1 H2]". iApply "H1". done.
       + eapply holds_entails. 2: apply Hrest; naive_solver.
         eauto.
-  Admitted.
+  Qed.
+
+  Lemma inv_delete (v1 v2 : V) (f f' : V -> multiset L -> hProp V L) :
+    (∀ v, Proper ((≡) ==> (⊣⊢)) (f v)) ->
+    (∀ v x, v ≠ v1 ∧ v ≠ v2 -> f v x ⊢ f' v x) ->
+    (∀ y, f v1 y ⊢ ∃ l,
+      own_out v2 l ∗
+      (∀ x,
+        f v2 ({[ l ]} ⋅ x) -∗
+          f' v1 y ∗
+          f' v2 x)) ->
+    inv f -> inv f'.
+  Proof.
+    intros Hproper Hrest Hexch Hinv.
+    unfold inv in *.
+    destruct Hinv as (g & Hwf & Hvs).
+    pose proof (Hvs v1) as Hv1.
+    specialize (Hexch (in_labels g v1)).
+    eapply holds_entails in Hexch; last done.
+    apply exists_holds in Hexch as (b & HH).
+    apply sep_holds in HH as (Σ1 & Σ2 & HΣ12 & H1 & H2 & H3).
+    apply own_holds in H2. subst.
+
+    assert (out_edges g v1 !! v2 = Some b) as Hv1outv2. {
+      rewrite HΣ12. rewrite lookup_union lookup_singleton.
+      destruct (_ !! _); eauto.
+    }
+
+    pose proof (Hvs v2) as Hv2.
+    assert (out_edges g v1 ##ₘ out_edges g v2) as Hdisj_out
+      by eauto using edge_out_disjoint, some_edge.
+
+    assert (Σ2 ##ₘ out_edges g v2) as Hdisj. {
+      rewrite HΣ12 in Hdisj_out.
+      solve_map_disjoint.
+    }
+
+    assert (∃ x, in_labels g v2 ≡ {[ b ]} ⋅ x) as [x Hx].
+      by by eapply out_edges_in_labels.
+
+    pose proof (sep_combine _ _ _ _ H3 Hv2 Hdisj) as Hcomb.
+    eapply holds_entails in Hcomb. 2: {
+      iIntros "[H1 H2]".
+      rewrite Hx.
+      iApply ("H1" with "H2").
+    }
+
+    apply sep_holds in Hcomb as (Σ1' & Σ2' & HΣ12' & Hdisj' & H1' & H2').
+
+    assert (v1 ≠ v2). {
+      intros ->. specialize (Hdisj_out v2). by rewrite Hv1outv2 in Hdisj_out.
+    }
+
+    assert (dealloc_valid g v1 v2 Σ1' Σ2'). {
+      unfold dealloc_valid. split_and!.
+      - eauto using some_edge.
+      - solve_map_disjoint.
+      - rewrite HΣ12.
+        rewrite delete_union delete_singleton left_id_L.
+        rewrite delete_notin; eauto.
+        solve_map_disjoint.
+    }
+
+    exists (dealloc g v1 v2 Σ1' Σ2').
+    split.
+    - apply dealloc_wf; eauto.
+    - intros v.
+      erewrite dealloc_out_edges.
+      setoid_rewrite dealloc_in_labels; eauto.
+      repeat case_decide; simplify_eq; eauto.
+      eapply holds_entails. 2: apply Hrest; naive_solver.
+      eauto.
+  Qed.
+
+  Lemma inv_insert_l (v1 v2 : V) (f f' : V -> multiset L -> hProp V L) :
+    (* (∀ v, Proper ((≡) ==> (⊣⊢)) (f v)) -> *)
+    (∀ v x, v ≠ v1 ∧ v ≠ v2 -> f v x ⊢ f' v x) ->
+    (∀ x, f v2 x ⊢ ⌜⌜ x ≡ ε ⌝⌝) ->
+    (∀ y, f v1 y ⊢
+      ∃ l',
+        (own_out v2 l' -∗ f' v1 y) ∗
+        f' v2 {[ l' ]}) ->
+    inv f -> inv f'.
+  Proof. Admitted.
+
+  Lemma inv_insert_r (v2 v3 : V) (f f' : V -> multiset L -> hProp V L) :
+    (* (∀ v, Proper ((≡) ==> (⊣⊢)) (f v)) -> *)
+    (∀ v x, v ≠ v3 ∧ v ≠ v2 -> f v x ⊢ f' v x) ->
+    (∀ x, f v3 x ⊢ ⌜⌜ x ≡ ε ⌝⌝) ->
+    (∀ y, f v2 y ⊢
+        ∃ l',
+          (own_out v2 l' -∗ f' v3 ε) ∗
+          f' v2 (y ⋅ {[ l' ]} )) ->
+    inv f -> inv f'.
+  Proof. Admitted.
+
+  Lemma inv_insert_lr (v1 v2 v3 : V) (f f' : V -> multiset L -> hProp V L) :
+    (* (∀ v, Proper ((≡) ==> (⊣⊢)) (f v)) -> *)
+    v1 ≠ v2 ∧ v2 ≠ v3 ∧ v3 ≠ v1 ->
+    (∀ v x, v ≠ v1 ∧ v ≠ v2 ∧ v ≠ v3 -> f v x ⊢ f' v x) ->
+    (∀ x, f v2 x ⊢ ⌜⌜ x ≡ ε ⌝⌝) ->
+    (∀ x, f v3 x ⊢ ⌜⌜ x ≡ ε ⌝⌝) ->
+    (∀ y, f v1 y ⊢
+      ∃ l1' l2',
+        (own_out v2 l1' -∗ f' v1 y) ∗
+        f' v2 ({[ l1' ]} ⋅ {[ l2' ]}) ∗
+        (own_out v2 l2' -∗ f' v3 ε)) ->
+    inv f -> inv f'.
+  Proof.
+    intros (Hneq1 & Hneq2 & Hneq3) Hrest H2 H3 H1 Hinv.
+    assert (inv (λ v x,
+      if decide (v = v1) then f' v1 x
+      else if decide (v = v2) then ∃ l2', f' v2 (x ⋅ {[l2']}) ∗ (own_out v2 l2' -∗ f' v3 ε)
+      else f v x))%I.
+    - eapply (inv_insert_l v1 v2); last done; eauto.
+      + intros. iIntros "H". repeat case_decide; naive_solver.
+      + iIntros (y) "H".
+        iDestruct (H1 with "H") as (l1' l2') "[H1 H2]".
+        repeat case_decide; simplify_eq.
+        iExists l1'. iFrame.
+        iExists l2'. iFrame.
+    - eapply (inv_insert_r v2 v3); last done.
+      + intros. simpl. destruct H4.
+        repeat case_decide; simplify_eq; eauto.
+      + intros; simpl. repeat case_decide; simplify_eq; eauto.
+      + intros. simpl.
+        repeat case_decide; simplify_eq.
+        iIntros "H".
+        iDestruct "H" as (l2') "[H1 H2]".
+        iExists _. iFrame.
+  Qed.
+
 End genericinv.
