theories/todo.md
@@ -1,7 +1,7 @@
 * (? of ?) prove connectivity graph lemmas
-* (1 of 3) think about different way to do generic invariant and separation logic
-* (1 of 3) using those prove the generic invariant lemmas
-* (0.8 of 5) prove preservation using generic invariant library
+* (5 of 5) state the generic invariant lemmas
+* (3 of 5) prove the generic invariant lemmas
+* (5 of 5) prove preservation using generic invariant library
 * (0 of ∞) figure out adequacy statement for generic invariant
 * (0 of ∞) prove progress using that adequacy statement
 * extensions
